Flapjack.lean
@@ -46,6 +46,7 @@ import Flapjack.PanEval
 import Flapjack.Pancake.Semantics.PanSem
 import Flapjack.Pancake.Semantics.PanSem.LookupCode
 import Flapjack.Pancake.Semantics.ByteAlignBridge
+import Flapjack.Pancake.Semantics.LoopProps
 import Flapjack.PanObservationalSemantics
 import Flapjack.PanHHandleCallRet
 import Flapjack.PanMrec
